PLC/PLC_proofs.v
@@ -5,8 +5,17 @@ Require Export PLC_inf.
 (* Notations *)
 Notation "[ e2 / x ] e1" := (subst_term e2 x e1) (at level 25).
 Notation "e1 '→' e2" := (red1 e1 e2) (at level 20).
+(* Notation "e1 '→⋆' e2" := (clos_refl_trans _ red1 e1 e2) (at level 20). *)
 Notation "e1 '⇒' e2" := (para_red e1 e2) (at level 20).
 Notation "e1 '⋆' = e2" := (can e1 e2) (at level 20).
+
+(* Tactics *)
+Tactic Notation "absurdity" "with" tactic(tac) :=
+  assert False by tac; contradiction.
+Ltac absurdity := absurdity with auto.
+Ltac size_absurd size t :=
+  assert (1 <= size t) by auto with lngen; absurdity with omega.
+Ltac size_term_absurd t := size_absurd size_term t.
 
 (* Mutual induction principles *)
 Scheme pval_mut_ind_aux := Induction for pval Sort Prop
@@ -61,10 +70,6 @@ Qed.
 Lemma para_red_regular2 : forall e1 e2, e1 ⇒ e2 -> lc_term e2.
 Proof.
 intros e1 e2 H; induction H; eauto.
-pick fresh x.
-replace (open_term_wrt_term e1' e2') with e1'.
-  eauto.
-  symmetry; eauto with lngen.
 Qed.
 Hint Resolve para_red_regular1 para_red_regular2.
 
@@ -76,11 +81,53 @@ Qed.
 Lemma can_regular2 : forall e1 e2, e1⋆ = e2 -> lc_term e2.
 Proof.
 intros e1 e2 H; induction H; auto.
-pick fresh x; replace (open_term_wrt_term e1' e2') with e1'.
-  eauto.
-  symmetry; eauto with lngen.
+pick fresh x; auto with lngen.
+Qed.
+Hint Resolve can_regular1 can_regular2.
+
+Lemma can_renaming : forall e1 e2 x y,
+  e1 ⋆ = e2 ->
+  (subst_term (term_var_f y)  x e1) ⋆ = (subst_term (term_var_f y) x e2).
+Proof.
+assert (forall n e1, size_term e1 <= n -> forall e2 (x y: termvar),
+  can e1 e2 -> can (subst_term (term_var_f y) x e1) (subst_term (term_var_f y) x e2)) as Th.
+intro n; induction n; intros e1 Hsize e2 x y H.
+size_term_absurd e1.
+destruct H; simpl in *.
+Case "var". destruct (x0 == x); subst; auto.
+Case "abs". apply can_abs with (L := L `union` {{ x }}); intros.
+  replace (term_var_f x0) with (subst_term (term_var_f y) x (term_var_f x0)) by auto with lngen.
+  repeat rewrite <- subst_term_open_term_wrt_term; auto.
+  apply IHn; auto; autorewrite with lngen; omega.
+Case "app1". apply can_app1; try solve [apply IHn; auto; omega].
+  intro; destruct e1; simpl; try congruence. destruct (t == x); congruence.
+Case "app2".
+  rewrite subst_term_open_term_wrt_term; auto.
+  apply can_app2 with (L := L `union` {{x}}); intros.
+  replace (term_var_f x0) with (subst_term (term_var_f y) x (term_var_f x0)) by auto with lngen.
+  repeat rewrite <- subst_term_open_term_wrt_term; auto.
+  apply IHn; auto; autorewrite with lngen; omega.
+  apply IHn; auto; omega.
+
+intros e1 e2 x y H; apply Th with (n := size_term e1); auto.
 Qed.
 
+(* Lemmas about values *)
+Lemma value_is_normal_aux :
+  (forall v, pval v -> ~ exists e, v → e) /\
+  (forall v, val v -> ~ exists e, v → e).
+Proof.
+apply pval_val_mut_ind; intros; intros [e0 Hred]; inversion Hred; subst; eauto.
+inversion H.
+inversion H1; subst. inversion p.
+inversion H0.
+pick fresh x. eapply H; eauto.
+Qed.
+
+Lemma value_is_normal : forall v, val v -> ~ exists e, v → e.
+Proof.
+destruct value_is_normal_aux as [_ Th]. intuition auto.
+Qed.
 
 (* Lemmas about canonize *)
 Lemma can_deterministic : forall e e1 e2,
@@ -92,12 +139,29 @@ inversion H1; subst; f_equal; pick fresh x;
   apply open_term_wrt_term_inj with (x1 := x); auto.
 inversion H2; subst.
   erewrite IHcan1; eauto; erewrite IHcan2; eauto.
-  destruct H; eauto.
+  edestruct H; eauto.
 inversion H2; subst.
-  destruct H5; eauto.
-  pick fresh x; erewrite H0; eauto; erewrite IHcan; eauto.
+  edestruct H5; eauto.
+  f_equal; auto.
+  pick fresh x; eauto using open_term_wrt_term_inj.
 Qed.
 
+Lemma can_total : forall e1, lc_term e1 -> exists e2, e1⋆ = e2.
+Proof.
+intros e1 Hlc; induction Hlc; eauto.
+Case "abs". pick fresh x; destruct (H0 x) as [e2 H2].
+  exists (term_abs (close_term_wrt_term x e2)).
+  apply can_abs with (L := {{x}}); intros.
+  rewrite <- (close_term_wrt_term_open_term_wrt_term e x); auto.
+  repeat rewrite <- subst_term_spec.
+  auto using can_renaming.
+Case "app". destruct IHHlc1 as [e1' H1]. destruct IHHlc2 as [e2' H2].
+destruct Hlc1; try solve [exists (term_app e1' e2'); apply can_app1; auto; congruence].
+SCase "abs".
+inversion H1; subst. exists (open_term_wrt_term e' e2'). apply can_app2 with (L := L); auto.
+Qed.
+
+(*
 Lemma can_fv : forall e1 e2, e1⋆ = e2 -> fv_term e2 [<=] fv_term e1.
 Proof.
 intros e1 e2 H; induction H; simpl; try fsetdec.
@@ -113,17 +177,154 @@ Case "app1".
 Case "app2".
   assert (fv_term (open_term_wrt_term e1' e2')
     [<=] union (fv_term e2') (fv_term e1')) by auto with lngen.
-  pick fresh x.
-  intros y Hy.
-  assert (y `in` union (fv_term e2') (fv_term e1')) as Hy' by auto.
-(* ICI *)
-  apply union_1 in Hy'; destruct Hy'.
-    assert (y = x) by fsetdec termvar; subst; assert False by fsetdec termvar; contradiction.
-    assumption.
-assert (fv_ex (open_ex t2' t1') [<=] fv_ex t2' `union` fv_ex t1') by auto with lngen.
-  fsetdec termvar.
+  intros y Hy. pick fresh x.
+  assert (fv_term e1' [<=] fv_term (open_term_wrt_term e1' (term_var_f x))) as H3 by auto with lngen.
+  assert (fv_term (open_term_wrt_term e1 (term_var_f x)) [<=] fv_term (term_var_f x) `union` fv_term e1) as H4 by auto with lngen.
+  assert (fv_term (open_term_wrt_term e1' (term_var_f x)) [<=] fv_term (open_term_wrt_term e1 (term_var_f x))) as H5 by auto.
+  assert (fv_term e1' [<=] fv_term (term_var_f x) `union` fv_term e1) as H6 by fsetdec; clear H3 H4 H5.
+  assert (y `in` fv_term (term_var_f x) `union` fv_term e1 `union` fv_term e2) as H3 by fsetdec; clear H6.
+  simpl in *; fsetdec.
+Qed.
+Hint Resolve can_fv.
+*)
 
-Lemma can_total : forall e1, lc_term e1 -> exists e2, e1⋆ = e2.
+(* Lemmas about red_star *)
+(*
+Lemma red_star_context_app : forall e1 e1' e2 e2',
+  lc_term e1 -> lc_term e2 ->
+  e1 →⋆ e1' -> e2 →⋆ e2' ->
+  term_app e1 e2 →⋆ term_app e1' e2'.
 Proof.
-intros e1 Hlc; induction Hlc; eauto.
-pick fresh x. destruct (H0 x) as [e2 H2]. exists (term_abs e2).
+(* TODO *)
+Admitted.
+*)
+
+
+(* Lemmas about para_red *)
+Lemma para_red_refl : forall e, lc_term e -> e ⇒ e.
+Proof.
+intros e H. induction H; try solve [constructor; auto].
+apply para_red_abs with (L := fv_term e); auto.
+Qed.
+Hint Resolve para_red_refl.
+
+Lemma red0_para_red : forall e1 e2, red0 e1 e2 -> e1 ⇒ e2.
+Proof.
+intros e1 e2 H. inversion H; subst.
+apply para_red_app2 with (L := fv_term e0); eauto.
+Qed.
+Hint Resolve red0_para_red.
+
+Lemma red1_para_red : forall e1 e2, e1 → e2 -> e1 ⇒ e2.
+Proof.
+intros e1 e2 H. induction H; auto.
+apply para_red_abs with (L := L); auto.
+Qed.
+
+Lemma para_red_subst : forall e1 e1' e2 e2' x,
+  e1 ⇒ e1' -> e2 ⇒ e2' ->
+  (subst_term e2 x e1) ⇒ (subst_term e2' x e1').
+Proof.
+intros e1 e1' e2 e2' x H.
+assert (lc_term e1) as Hlc by eauto.
+generalize dependent e1'.
+generalize dependent e2.
+generalize dependent e2'.
+generalize dependent x.
+induction Hlc; intros y f2' f2 e1' Htt' Huu'; inversion Htt'; subst; simpl.
+destruct (x == y); auto.
+apply para_red_abs with (L := L `union` singleton y); intros.
+  assert (term_var_f x = subst_term f2 y (term_var_f x)) as H3. autorewrite with lngen; reflexivity.
+  assert (term_var_f x = subst_term f2' y (term_var_f x)) as H4. autorewrite with lngen; reflexivity.
+  rewrite H3 at 1; clear H3.
+  rewrite H4 at 2; clear H4.
+  repeat rewrite <- subst_term_open_term_wrt_term; eauto.
+apply para_red_app1; auto.
+rewrite subst_term_open_term_wrt_term; eauto.
+  assert (para_red (subst_term f2 y (term_abs e0)) (subst_term f2' y (term_abs e1'0))) as Ht.
+    apply IHHlc1; auto;
+    apply para_red_abs with (L := L); auto.
+  simpl in Ht; inversion Ht; subst; clear Ht.
+  apply para_red_app2 with (L := L `union` L0 `union` {{y}}); auto.
+Qed.
+
+Lemma para_red_canonize : forall e1 e2 e1',
+  e1 ⇒ e2 -> e1 ⋆ = e1' -> e2 ⇒ e1'.
+Proof.
+intros e1 e2 e1' Hpara Hcan. generalize dependent e1'.
+induction Hpara; intros v Hcan.
+inversion Hcan; subst; constructor.
+inversion Hcan; subst; apply para_red_abs with (L := L `union` L0); intros; auto.
+inversion Hcan; subst.
+  constructor; auto.
+  inversion Hpara1; subst; pick fresh x; assert (para_red (term_abs e') (term_abs e1'0)) as H by eauto.
+    inversion H; subst; apply para_red_app2 with (L := L1); intros; auto.
+inversion Hcan; subst.
+  absurdity with congruence.
+  pick fresh x for (fv_term e1' `union` fv_term e1'0 `union` L `union` L0).
+  rewrite <- (close_term_wrt_term_open_term_wrt_term e1' x); auto.
+  rewrite <- (close_term_wrt_term_open_term_wrt_term e1'0 x); auto.
+  repeat rewrite <- subst_term_spec.
+  apply para_red_subst; auto.
+Qed.
+
+Lemma para_red_diamond : forall e e1 e2,
+  e ⇒ e1 -> e ⇒ e2 -> exists e', e1 ⇒ e' /\ e2 ⇒ e'.
+Proof.
+intros e e1 e2 H1 H2.
+destruct (can_total e) as [e' H']; eauto.
+eauto using para_red_canonize.
+Qed.
+
+(*
+Lemma para_red_red_star : forall e1 e2, e1 ⇒ e2 -> e1 →⋆ e2.
+Proof.
+intros e1 e2 H.
+assert (lc_term e1) as Hlc by eauto.
+generalize dependent e2.
+induction Hlc; intros e0 Hpara; inversion Hpara; subst.
+apply rt_refl.
+pick fresh x for (L `union` fv_term e `union` fv_term e').
+  assert (open_term_wrt_term e (term_var_f x) ⇒ open_term_wrt_term e' (term_var_f x)) by auto.
+  assert (open_term_wrt_term e (term_var_f x) →⋆ open_term_wrt_term e' (term_var_f x)) by auto.
+(* TODO *)
+
+  assert (red_star (open_ex x e) (open_ex x e20)) as Hpara' by auto.
+  replace (term_abs e) with (inject (CAbs x CEmpty) (open_ex x e)).
+  replace (term_abs e20) with (inject (CAbs x CEmpty) (open_ex x e20)).
+  apply red_star_context_closed; auto.
+  simpl; rewrite close_ex_open_ex; auto.
+  simpl; rewrite close_ex_open_ex; auto.
+assert (red_star e e20) as He by auto. assert (red_star e1 u') as He1 by auto.
+  clear IHHlc1 IHHlc2 H1 H3 Hpara.
+  inversion He; subst.
+    replace (term_app e20 e1) with (inject (CAppR e20 CEmpty) e1) by reflexivity.
+    replace (term_app e20 u') with (inject (CAppR e20 CEmpty) u') by reflexivity.
+    apply red_star_context_closed; auto.
+  inversion He1; subst.
+    replace (term_app e u') with (inject (CAppL CEmpty u') e) by reflexivity.
+    replace (term_app e20 u') with (inject (CAppL CEmpty u') e20) by reflexivity.
+    apply red_star_context_closed; auto.
+  apply red_star_trans with (t2 := term_app e20 e1).
+    replace (term_app e e1) with (inject (CAppL CEmpty e1) e) by reflexivity.
+    replace (term_app e20 e1) with (inject (CAppL CEmpty e1) e20) by reflexivity.
+    apply red_star_context_closed; auto.
+    replace (term_app e20 e1) with (inject (CAppR e20 CEmpty) e1) by reflexivity.
+    replace (term_app e20 u') with (inject (CAppR e20 CEmpty) u') by reflexivity.
+    apply red_star_context_closed; auto.
+assert (red_star (term_abs e1) (term_abs e20)) as Ht.
+    apply IHHlc1. apply ParaAbs with (S := S `union` fv_term e1 `union` fv_term e1 `union` fv_term u' `union` fv_term e20). auto.
+  assert (red_star e1 u') as He1 by auto.
+  apply red_star_trans with (t2 := term_app (term_abs e20) e1).
+    replace (term_app (term_abs e1) e1) with (inject (CAppL CEmpty e1) (term_abs e1)) by reflexivity.
+    replace (term_app (term_abs e20) e1) with (inject (CAppL CEmpty e1) (term_abs e20)) by reflexivity.
+    apply red_star_context_closed; auto.
+  apply red_star_trans with (t2 := term_app (term_abs e20) u').
+    replace (term_app (term_abs e20) e1) with (inject (CAppR (term_abs e20) CEmpty) e1) by reflexivity.
+    replace (term_app (term_abs e20) u') with (inject (CAppR (term_abs e20) CEmpty) u') by reflexivity.
+    apply red_star_context_closed; auto.
+    replace (term_app (term_abs e20) u') with (inject CEmpty (term_app (term_abs e20) u')) by reflexivity.
+    replace (open_ex u' e20) with (inject CEmpty (open_ex u' e20)) by reflexivity.
+    apply RedSome. apply RedOne. constructor. constructor.
+Qed.
+*)
